src/iopt/iSplitRel.v
@@ -21,29 +21,30 @@ Require Import SimMemory.
 Require Import SimPromises.
 Require Import SimLocal.
 Require Import SimThread.
-Require Import Compatibility.
+Require Import iCompatibility.
 Require Import SplitRelCommon.
 
-Require Import Syntax.
-Require Import Semantics.
+Require Import ITreeLang.
 
 Set Implicit Arguments.
 
 
-Inductive split_release: forall (i1 i2:Instr.t), Prop :=
+Inductive split_release: forall R (i1: MemE.t R) (i2: MemE.t R), Prop :=
 | split_release_store
     l v:
-    split_release (Instr.store l v Ordering.acqrel) (Instr.store l v Ordering.strong_relaxed)
+    split_release (MemE.write l v Ordering.acqrel) (MemE.write l v Ordering.strong_relaxed)
 | split_release_update
-    r l rmw or
+    l rmw or
     (OR: Ordering.le or Ordering.strong_relaxed):
-    split_release (Instr.update r l rmw or Ordering.acqrel) (Instr.update r l rmw or Ordering.strong_relaxed)
+    split_release (MemE.update l rmw or Ordering.acqrel) (MemE.update l rmw or Ordering.strong_relaxed)
 .
 
-Inductive sim_released: forall (st_src:(Language.state lang)) (lc_src:Local.t) (sc1_src:TimeMap.t) (mem1_src:Memory.t)
-                          (st_tgt:(Language.state lang)) (lc_tgt:Local.t) (sc1_tgt:TimeMap.t) (mem1_tgt:Memory.t), Prop :=
+Inductive sim_released: forall R
+                               (st_src:(Language.state (lang R))) (lc_src:Local.t) (sc1_src:TimeMap.t) (mem1_src:Memory.t)
+                               (st_tgt:(Language.state (lang R))) (lc_tgt:Local.t) (sc1_tgt:TimeMap.t) (mem1_tgt:Memory.t), Prop :=
 | sim_released_intro
-    i_src i_tgt rs
+    R
+    (i_src i_tgt: MemE.t R)
     lc1_src sc1_src mem1_src
     lc1_tgt sc1_tgt mem1_tgt
     (SPLIT: split_release i_src i_tgt)
@@ -58,11 +59,12 @@ Inductive sim_released: forall (st_src:(Language.state lang)) (lc_src:Local.t) (
     (MEM_SRC: Memory.closed mem1_src)
     (MEM_TGT: Memory.closed mem1_tgt):
     sim_released
-      (State.mk rs [Stmt.instr i_src]) lc1_src sc1_src mem1_src
-      (State.mk rs [Stmt.instr i_tgt]) lc1_tgt sc1_tgt mem1_tgt
+      (Vis i_src (fun r => Ret r)) lc1_src sc1_src mem1_src
+      (Vis i_tgt (fun r => Ret r)) lc1_tgt sc1_tgt mem1_tgt
 .
 
 Lemma sim_released_mon
+      R
       st_src lc_src sc1_src mem1_src
       st_tgt lc_tgt sc1_tgt mem1_tgt
       sc2_src mem2_src
@@ -81,24 +83,26 @@ Lemma sim_released_mon
       (SC_TGT: Memory.closed_timemap sc2_tgt mem2_tgt)
       (MEM_SRC: Memory.closed mem2_src)
       (MEM_TGT: Memory.closed mem2_tgt):
-  sim_released st_src lc_src sc2_src mem2_src
-               st_tgt lc_tgt sc2_tgt mem2_tgt.
+  @sim_released R
+                st_src lc_src sc2_src mem2_src
+                st_tgt lc_tgt sc2_tgt mem2_tgt.
 Proof.
-  inv SIM1. econs; eauto.
+  destruct SIM1. econs; eauto.
 Qed.
 
-Lemma sim_released_step
+Lemma sim_released_step R
       st1_src lc1_src sc1_src mem1_src
       st1_tgt lc1_tgt sc1_tgt mem1_tgt
-      (SIM: sim_released st1_src lc1_src sc1_src mem1_src
-                         st1_tgt lc1_tgt sc1_tgt mem1_tgt):
-  _sim_thread_step lang lang ((sim_thread (sim_terminal eq)) \8/ sim_released)
+      (SIM: @sim_released R
+                          st1_src lc1_src sc1_src mem1_src
+                          st1_tgt lc1_tgt sc1_tgt mem1_tgt):
+  _sim_thread_step (lang R) (lang R)
+                   ((@sim_thread (lang R) (lang R) (sim_terminal eq)) \8/ @sim_released R)
                    st1_src lc1_src sc1_src mem1_src
                    st1_tgt lc1_tgt sc1_tgt mem1_tgt.
 Proof.
-  inv SIM. ii.
-  inv STEP_TGT; [inv STEP|inv STEP; inv LOCAL0];
-    try (inv STATE; inv INSTR; inv SPLIT); ss.
+  destruct SIM. ii.
+  inv STEP_TGT; [inv STEP|dependent destruction STEP; inv LOCAL0; ss; dependent destruction STATE; inv SPLIT]; ss.
   - (* promise *)
     right.
     exploit Local.promise_step_future; eauto. i. des.
@@ -109,14 +113,16 @@ Proof.
     + eauto.
     + right. econs; eauto.
       inv LOCAL0. ss.
-  - (* update-load *)
+  - dependent destruction H.
+    (* update-load *)
     right.
     exploit sim_local_read; (try by etrans; eauto); eauto; try refl. i. des.
     esplits; eauto; ss.
-    + econs 2. econs 2. econs; [|econs 2]; eauto. econs. econs. eauto.
+    + econs 2. econs 2. econs; [|econs 2]; eauto. econs; eauto.
     + eauto.
-    + left. eapply paco11_mon; [apply sim_stmts_nil|]; ss.
-  - (* write *)
+    + left. eapply paco11_mon; [apply sim_itree_ret|]; ss.
+  - dependent destruction H.
+    (* write *)
     right.
     hexploit sim_local_write_released; (try by etrans; eauto); eauto; try refl; try by econs.
     { by rewrite <- View.join_l. }
@@ -124,8 +130,9 @@ Proof.
     esplits; eauto; ss.
     + econs 2. econs 2. econs; [|econs 3]; eauto. econs. econs.
     + ss.
-    + left. eapply paco11_mon; [apply sim_stmts_nil|]; ss.
-  - (* update *)
+    + left. eapply paco11_mon; [apply sim_itree_ret|]; ss.
+  - dependent destruction H.
+    (* update *)
     right.
     exploit Local.read_step_future; eauto. i. des.
     exploit sim_local_read; (try by etrans; eauto); eauto; try refl; try by econs. i. des.
@@ -138,13 +145,13 @@ Proof.
     }
     i. des.
     esplits; eauto; ss.
-    + econs 2. econs 2. econs; [|econs 4]; eauto. econs. econs. eauto.
+    + econs 2. econs 2. econs; [|econs 4]; eauto. econs; eauto.
     + ss.
-    + left. eapply paco11_mon; [apply sim_stmts_nil|]; ss.
+    + left. eapply paco11_mon; [apply sim_itree_ret|]; ss.
 Qed.
 
-Lemma sim_released_sim_thread:
-  sim_released <8= (sim_thread (sim_terminal eq)).
+Lemma sim_released_sim_thread R:
+  @sim_released R <8= @sim_thread (lang R) (lang R) (sim_terminal eq).
 Proof.
   pcofix CIH. i. pfold. ii. ss. splits; ss; ii.
   - inv TERMINAL_TGT. inv PR; ss.
@@ -157,22 +164,20 @@ Proof.
     + right. esplits; eauto.
 Qed.
 
-Lemma split_release_sim_stmts
-      i_src i_tgt
+Lemma split_release_sim_itree R
+      (i_src i_tgt: MemE.t R)
       (SPLIT: split_release i_src i_tgt):
-  sim_stmts eq
-            [Stmt.instr i_src]
-            [Stmt.instr (Instr.fence Ordering.plain Ordering.acqrel); Stmt.instr i_tgt]
-            eq.
+  sim_itree eq
+            (Vis i_src (fun r => Ret r))
+            (Vis (MemE.fence Ordering.plain Ordering.acqrel) (fun _ => Vis i_tgt (fun r => Ret r))).
 Proof.
   pcofix CIH. ii. subst. pfold. ii. splits; ii.
-  { inv TERMINAL_TGT. }
+  { inv TERMINAL_TGT. eapply f_equal with (f:=observe) in H; ss. }
   { right. esplits; eauto.
     inv LOCAL. apply SimPromises.sem_bot_inv in PROMISES; auto. rewrite PROMISES. auto.
   }
   right.
-  inv STEP_TGT; [inv STEP|inv STEP; inv LOCAL0];
-    try (inv STATE; inv INSTR); ss.
+  inv STEP_TGT; [inv STEP|dependent destruction STEP; inv LOCAL0; ss; dependent destruction STATE]; ss.
   - (* promise *)
     exploit sim_local_promise; eauto. i. des.
     esplits; try apply SC; eauto; ss.
