src/opt_common/MergeStep.v
@@ -25,7 +25,6 @@ Require Import SimMemory.
 Require Import SimPromises.
 Require Import SimLocal.
 Require Import SimThread.
-Require Import Compatibility.
 
 Require Import MergeTView.
 
