src/opt_common/SplitAcqRelCommon.v
@@ -1,0 +1,193 @@
+From sflib Require Import sflib.
+From Paco Require Import paco.
+
+From PromisingLib Require Import Basic.
+From PromisingLib Require Import Loc.
+From PromisingLib Require Import Language.
+
+Require Import Event.
+Require Import Time.
+Require Import View.
+Require Import Cell.
+Require Import Memory.
+Require Import TView.
+Require Import Local.
+Require Import Thread.
+Require Import Configuration.
+
+Require Import FulfillStep.
+
+Require Import SimMemory.
+Require Import SimPromises.
+Require Import SimLocal.
+Require Import SimThread.
+
+Require Import SplitAcqCommon.
+
+Set Implicit Arguments.
+
+
+Definition local_acqrel (lc:Local.t) :=
+  (Local.mk (TView.write_fence_tview
+               (TView.read_fence_tview (Local.tview lc) Ordering.acqrel)
+               TimeMap.bot
+               Ordering.acqrel)
+            (Local.promises lc)).
+
+Lemma sim_local_promise_acqrel
+      lc1_src mem1_src
+      lc1_tgt mem1_tgt
+      lc2_tgt mem2_tgt
+      loc from to msg kind
+      (STEP_TGT: Local.promise_step lc1_tgt mem1_tgt loc from to msg lc2_tgt mem2_tgt kind)
+      (LOCAL1: sim_local SimPromises.bot lc1_src (local_acqrel lc1_tgt))
+      (MEM1: sim_memory mem1_src mem1_tgt)
+      (WF1_SRC: Local.wf lc1_src mem1_src)
+      (WF1_TGT: Local.wf lc1_tgt mem1_tgt)
+      (MEM1_SRC: Memory.closed mem1_src)
+      (MEM1_TGT: Memory.closed mem1_tgt):
+  exists lc2_src mem2_src,
+    <<STEP_SRC: Local.promise_step lc1_src mem1_src loc from to msg lc2_src mem2_src kind>> /\
+    <<LOCAL2: sim_local SimPromises.bot lc2_src (local_acqrel lc2_tgt)>> /\
+    <<MEM2: sim_memory mem2_src mem2_tgt>>.
+Proof.
+  inv LOCAL1. inv STEP_TGT.
+  exploit SimPromises.promise_bot; eauto.
+  { apply WF1_SRC. }
+  { apply WF1_TGT. }
+  i. des.
+  exploit Memory.promise_future; try apply PROMISE_SRC; try apply WF1_SRC; eauto.
+  { destruct msg; ss. inv CLOSED. econs.
+    eapply sim_memory_closed_opt_view; eauto. }
+  i. des.
+  esplits; eauto.
+  - econs; eauto.
+    destruct msg; ss. inv CLOSED. econs.
+    eapply sim_memory_closed_opt_view; eauto.
+  - econs; eauto.
+Qed.
+
+Lemma sim_local_fulfill_acqrel
+      lc1_src sc1_src mem1_src
+      lc1_tgt sc1_tgt mem1_tgt
+      lc2_tgt sc2_tgt
+      loc from to val releasedm_src releasedm_tgt released ord_src ord_tgt
+      (RELM_LE: View.opt_le releasedm_src releasedm_tgt)
+      (RELM_WF: View.opt_wf releasedm_src)
+      (RELM_CLOSED: Memory.closed_opt_view releasedm_src mem1_src)
+      (RELM_TGT: Time.le (View.rlx (View.unwrap releasedm_tgt) loc) from)
+      (WF_RELM_TGT: View.opt_wf releasedm_tgt)
+      (ORD: Ordering.le ord_src ord_tgt)
+      (ORD_TGT: Ordering.le ord_tgt Ordering.acqrel)
+      (STEP_TGT: fulfill_step lc1_tgt sc1_tgt loc from to val releasedm_tgt released ord_tgt lc2_tgt sc2_tgt)
+      (LOCAL1: sim_local SimPromises.bot lc1_src (local_acquired lc1_tgt))
+      (ACQUIRED1: View.le (TView.cur (Local.tview lc1_src))
+                          (View.join (TView.cur (Local.tview lc1_tgt)) (View.unwrap releasedm_tgt)))
+      (SC1: TimeMap.le sc1_src sc1_tgt)
+      (MEM1: sim_memory mem1_src mem1_tgt)
+      (WF1_SRC: Local.wf lc1_src mem1_src)
+      (WF1_TGT: Local.wf lc1_tgt mem1_tgt)
+      (SC1_SRC: Memory.closed_timemap sc1_src mem1_src)
+      (SC1_TGT: Memory.closed_timemap sc1_tgt mem1_tgt)
+      (MEM1_SRC: Memory.closed mem1_src)
+      (MEM1_TGT: Memory.closed mem1_tgt):
+  exists lc2_src sc2_src,
+    <<STEP_SRC: fulfill_step lc1_src sc1_src loc from to val releasedm_src released ord_src lc2_src sc2_src>> /\
+    <<LOCAL2: sim_local SimPromises.bot lc2_src (local_acqrel lc2_tgt)>> /\
+    <<SC2: TimeMap.le sc2_src sc2_tgt>>.
+Proof.
+  inv STEP_TGT.
+  assert (RELT_LE:
+   View.opt_le
+     (TView.write_released (Local.tview lc1_src) sc1_src loc to releasedm_src ord_src)
+     (TView.write_released (Local.tview lc1_tgt) sc2_tgt loc to releasedm_tgt ord_tgt)).
+  { unfold TView.write_released, TView.write_tview. ss. viewtac.
+    repeat (condtac; aggrtac;
+            try match goal with
+                | [|- View.opt_le _ _] => econs
+                end);
+      try apply WF1_TGT.
+    - etrans; eauto. aggrtac.
+    - etrans; [apply WF1_SRC|]. etrans; eauto. aggrtac.
+    - etrans; [apply LOCAL1|]. aggrtac.
+  }
+  assert (RELT_WF:
+   View.opt_wf (TView.write_released (Local.tview lc1_src) sc1_src loc to releasedm_src ord_src)).
+  { unfold TView.write_released. condtac; econs.
+    repeat (try condtac; viewtac; try apply WF1_SRC).
+  }
+  exploit SimPromises.remove_bot; try exact REMOVE;
+    try exact MEM1; try apply LOCAL1; eauto.
+  { econs. ss. }
+  { apply WF1_SRC. }
+  { apply WF1_TGT. }
+  { apply WF1_TGT. }
+  i. des. esplits.
+  - econs; eauto.
+    inv WRITABLE. econs.
+    eapply TimeFacts.le_lt_lt; [apply ACQUIRED1|]. viewtac.
+    eapply TimeFacts.le_lt_lt; eauto.
+  - econs; eauto. s.
+    unfold TView.write_tview, TView.write_fence_tview, TView.read_fence_tview. ss.
+    econs; ss; repeat (condtac; aggrtac).
+    all: try by destruct ord_src, ord_tgt.
+    all: try by apply WF1_TGT.
+    + etrans; [apply LOCAL1|]. repeat (try condtac; aggrtac).
+    + etrans; [apply LOCAL1|]. aggrtac.
+      etrans; [apply WF1_TGT|]. etrans; [apply WF1_TGT|]. aggrtac.
+    + etrans; [apply LOCAL1|]. aggrtac.
+      etrans; [apply WF1_TGT|]. etrans; [apply WF1_TGT|]. aggrtac.
+    + etrans; [apply LOCAL1|]. repeat (try condtac; aggrtac).
+      etrans; [apply WF1_TGT|]. etrans; [apply WF1_TGT|]. aggrtac.
+    + etrans; [apply LOCAL1|]. ss. condtac; aggrtac.
+    + etrans; [apply LOCAL1|]. aggrtac.
+  - ss.
+Qed.
+
+Lemma sim_local_write_acqrel
+      lc1_src sc1_src mem1_src
+      lc1_tgt sc1_tgt mem1_tgt
+      lc2_tgt sc2_tgt mem2_tgt
+      loc from to val releasedm_src releasedm_tgt released_tgt ord_src ord_tgt kind
+      (RELM_LE: View.opt_le releasedm_src releasedm_tgt)
+      (RELM_SRC_WF: View.opt_wf releasedm_src)
+      (RELM_SRC_CLOSED: Memory.closed_opt_view releasedm_src mem1_src)
+      (RELM_TGT_WF: View.opt_wf releasedm_tgt)
+      (RELM_TGT_CLOSED: Memory.closed_opt_view releasedm_tgt mem1_tgt)
+      (RELM_TGT: Time.le (View.rlx (View.unwrap releasedm_tgt) loc) from)
+      (ORD: Ordering.le ord_src ord_tgt)
+      (ORD_TGT: Ordering.le ord_tgt Ordering.acqrel)
+      (STEP_TGT: Local.write_step lc1_tgt sc1_tgt mem1_tgt loc from to val releasedm_tgt released_tgt ord_tgt lc2_tgt sc2_tgt mem2_tgt kind)
+      (LOCAL1: sim_local SimPromises.bot lc1_src (local_acquired lc1_tgt))
+      (ACQUIRED1: View.le (TView.cur (Local.tview lc1_src))
+                          (View.join (TView.cur (Local.tview lc1_tgt)) (View.unwrap releasedm_tgt)))
+      (SC1: TimeMap.le sc1_src sc1_tgt)
+      (MEM1: sim_memory mem1_src mem1_tgt)
+      (WF1_SRC: Local.wf lc1_src mem1_src)
+      (WF1_TGT: Local.wf lc1_tgt mem1_tgt)
+      (SC1_SRC: Memory.closed_timemap sc1_src mem1_src)
+      (SC1_TGT: Memory.closed_timemap sc1_tgt mem1_tgt)
+      (MEM1_SRC: Memory.closed mem1_src)
+      (MEM1_TGT: Memory.closed mem1_tgt):
+  exists released_src lc2_src sc2_src mem2_src,
+    <<STEP_SRC: Local.write_step lc1_src sc1_src mem1_src loc from to val releasedm_src released_src ord_src lc2_src sc2_src mem2_src kind>> /\
+    <<REL2: View.opt_le released_src released_tgt>> /\
+    <<LOCAL2: sim_local SimPromises.bot lc2_src (local_acqrel lc2_tgt)>> /\
+    <<SC2: TimeMap.le sc2_src sc2_tgt>> /\
+    <<MEM2: sim_memory mem2_src mem2_tgt>>.
+Proof.
+  exploit write_promise_fulfill; eauto. i. des.
+  exploit Local.promise_step_future; eauto. i. des.
+  exploit sim_local_promise_acquired; eauto. i. des.
+  exploit Local.promise_step_future; eauto. i. des.
+  hexploit sim_local_fulfill_acqrel; try apply STEP2;
+    try apply LOCAL2; try apply MEM2; eauto.
+  { eapply Memory.future_closed_opt_view; eauto. }
+  { inv STEP_SRC. inv STEP1. ss. }
+  i. des.
+  exploit promise_fulfill_write_sim_memory; try exact STEP_SRC; try exact STEP_SRC0; eauto.
+  { i. hexploit ORD0; eauto.
+    i. des. splits; auto. eapply sim_local_nonsynch_loc; eauto.
+  }
+  i. des. esplits; eauto. etrans; eauto.
+Qed.
