src/opt_common/SplitRelCommon.v
@@ -1,0 +1,132 @@
+From sflib Require Import sflib.
+From Paco Require Import paco.
+
+From PromisingLib Require Import Basic.
+From PromisingLib Require Import Loc.
+From PromisingLib Require Import Language.
+
+Require Import Event.
+Require Import Time.
+Require Import View.
+Require Import Cell.
+Require Import Memory.
+Require Import TView.
+Require Import Local.
+Require Import Thread.
+Require Import Configuration.
+
+Require Import FulfillStep.
+
+Require Import SimMemory.
+Require Import SimPromises.
+Require Import SimLocal.
+Require Import SimThread.
+
+Set Implicit Arguments.
+
+
+Lemma sim_local_fulfill_released
+      lc1_src sc1_src mem1_src
+      lc1_tgt sc1_tgt mem1_tgt
+      lc2_tgt sc2_tgt
+      loc from to val releasedm_src releasedm_tgt released
+      (RELM_LE: View.opt_le releasedm_src releasedm_tgt)
+      (RELM_WF: View.opt_wf releasedm_src)
+      (RELM_CLOSED: Memory.closed_opt_view releasedm_src mem1_src)
+      (WF_RELM_TGT: View.opt_wf releasedm_tgt)
+      (STEP_TGT: fulfill_step lc1_tgt sc1_tgt loc from to val releasedm_tgt released Ordering.strong_relaxed lc2_tgt sc2_tgt)
+      (LOCAL1: sim_local SimPromises.bot lc1_src lc1_tgt)
+      (RELEASED1: View.le (TView.cur (Local.tview lc1_tgt)) (View.join ((TView.rel (Local.tview lc1_tgt)) loc) (View.singleton_ur loc to)))
+      (SC1: TimeMap.le sc1_src sc1_tgt)
+      (MEM1: sim_memory mem1_src mem1_tgt)
+      (WF1_SRC: Local.wf lc1_src mem1_src)
+      (WF1_TGT: Local.wf lc1_tgt mem1_tgt)
+      (SC1_SRC: Memory.closed_timemap sc1_src mem1_src)
+      (SC1_TGT: Memory.closed_timemap sc1_tgt mem1_tgt)
+      (MEM1_SRC: Memory.closed mem1_src)
+      (MEM1_TGT: Memory.closed mem1_tgt):
+  exists lc2_src sc2_src,
+    <<STEP_SRC: fulfill_step lc1_src sc1_src loc from to val releasedm_src released Ordering.acqrel lc2_src sc2_src>> /\
+    <<LOCAL2: sim_local SimPromises.bot lc2_src lc2_tgt>> /\
+    <<SC2: TimeMap.le sc2_src sc2_tgt>>.
+Proof.
+  inv STEP_TGT.
+  assert (RELT_LE:
+   View.opt_le
+     (TView.write_released (Local.tview lc1_src) sc1_src loc to releasedm_src Ordering.acqrel)
+     (TView.write_released (Local.tview lc1_tgt) sc2_tgt loc to releasedm_tgt Ordering.strong_relaxed)).
+  { unfold TView.write_released, TView.write_tview. ss. viewtac;
+      try econs; repeat (condtac; aggrtac); try apply WF1_TGT.
+    rewrite <- View.join_r. etrans; eauto. apply LOCAL1.
+  }
+  assert (RELT_WF:
+   View.opt_wf (TView.write_released (Local.tview lc1_src) sc1_src loc to releasedm_src Ordering.acqrel)).
+  { unfold TView.write_released. condtac; econs.
+    repeat (try condtac; viewtac; try apply WF1_SRC).
+  }
+  exploit SimPromises.remove_bot; try exact REMOVE;
+    try exact MEM1; try apply LOCAL1; eauto.
+  { econs. ss. }
+  { apply WF1_SRC. }
+  { apply WF1_TGT. }
+  { apply WF1_TGT. }
+  i. des. esplits.
+  - econs; eauto.
+    inv WRITABLE. econs; ss. eapply TimeFacts.le_lt_lt; [apply LOCAL1|apply TS].
+  - econs; eauto. s.
+    unfold TView.write_tview, View.singleton_ur_if. repeat (condtac; aggrtac).
+    econs; repeat (condtac; aggrtac);
+      (try by etrans; [apply LOCAL1|aggrtac]);
+      (try by rewrite <- ? View.join_r; econs; aggrtac);
+      (try apply WF1_TGT).
+    + ss. i. unfold LocFun.find. repeat (condtac; aggrtac).
+      * etrans; eauto. apply LOCAL1.
+      * apply LOCAL1.
+    + ss. aggrtac; try apply WF1_TGT. rewrite <- ? View.join_l. apply LOCAL1.
+    + ss. aggrtac; try apply WF1_TGT. rewrite <- ? View.join_l. apply LOCAL1.
+  - ss.
+Qed.
+
+Lemma sim_local_write_released
+      lc1_src sc1_src mem1_src
+      lc1_tgt sc1_tgt mem1_tgt
+      lc2_tgt sc2_tgt mem2_tgt
+      loc from to val releasedm_src releasedm_tgt released_tgt kind
+      (RELM_LE: View.opt_le releasedm_src releasedm_tgt)
+      (RELM_SRC_WF: View.opt_wf releasedm_src)
+      (RELM_SRC_CLOSED: Memory.closed_opt_view releasedm_src mem1_src)
+      (RELM_TGT_WF: View.opt_wf releasedm_tgt)
+      (RELM_TGT_CLOSED: Memory.closed_opt_view releasedm_tgt mem1_tgt)
+      (STEP_TGT: Local.write_step lc1_tgt sc1_tgt mem1_tgt loc from to val releasedm_tgt released_tgt Ordering.strong_relaxed lc2_tgt sc2_tgt mem2_tgt kind)
+      (LOCAL1: sim_local SimPromises.bot lc1_src lc1_tgt)
+      (RELEASED1: View.le (TView.cur (Local.tview lc1_tgt)) (View.join ((TView.rel (Local.tview lc1_tgt)) loc) (View.singleton_ur loc to)))
+      (SC1: TimeMap.le sc1_src sc1_tgt)
+      (MEM1: sim_memory mem1_src mem1_tgt)
+      (WF1_SRC: Local.wf lc1_src mem1_src)
+      (WF1_TGT: Local.wf lc1_tgt mem1_tgt)
+      (SC1_SRC: Memory.closed_timemap sc1_src mem1_src)
+      (SC1_TGT: Memory.closed_timemap sc1_tgt mem1_tgt)
+      (MEM1_SRC: Memory.closed mem1_src)
+      (MEM1_TGT: Memory.closed mem1_tgt):
+  exists released_src lc2_src sc2_src mem2_src,
+    <<STEP_SRC: Local.write_step lc1_src sc1_src mem1_src loc from to val releasedm_src released_src Ordering.acqrel lc2_src sc2_src mem2_src kind>> /\
+    <<REL2: View.opt_le released_src released_tgt>> /\
+    <<LOCAL2: sim_local SimPromises.bot lc2_src lc2_tgt>> /\
+    <<SC2: TimeMap.le sc2_src sc2_tgt>> /\
+    <<MEM2: sim_memory mem2_src mem2_tgt>>.
+Proof.
+  exploit write_promise_fulfill; eauto. i. des.
+  exploit Local.promise_step_future; eauto. i. des.
+  exploit sim_local_promise_bot; eauto. i. des.
+  exploit Local.promise_step_future; eauto. i. des.
+  exploit sim_local_fulfill_released; try apply STEP2;
+    try apply LOCAL2; try apply MEM2; eauto.
+  { eapply Memory.future_closed_opt_view; eauto. }
+  { by inv STEP1. }
+  i. des.
+  exploit promise_fulfill_write_sim_memory; try exact STEP_SRC; try exact STEP_SRC0; eauto.
+  { i. hexploit ORD; eauto. i. des. splits; ss.
+    eapply sim_local_nonsynch_loc; eauto.
+  }
+  i. des. esplits; eauto. etrans; eauto.
+Qed.
